studentapplication

studentapplication.bpl
@@ -1,39 +1,108 @@
+var college : [Ref]Ref;
+var campusNumber : [Ref]int;
+var facilities : [Ref]Ref;
 
+var packedStudentApplicationFields : [Ref]bool;
+var fracStudentApplicationFields : [Ref]real;
 
+var packedStudentAppFacilitiesMany : [Ref]bool;
+var fracStudentAppFacilitiesMany : [Ref]real;
 
+var packedStudentAppFacilitiesFew : [Ref]bool;
+var fracStudentAppFacilitiesFew : [Ref]real;
 
-class StudentApplication {
-College college; 
-int campusNumber; 
-IntCell facilities;
-int collegeNumber;
+procedure PackStudentApplicationFields(c:Ref, camp:int, fac:Ref, this:Ref);
+requires packedStudentApplicationFields[this] == false;
+requires (college[this] == c) && (campusNumber[this] == camp)
+	&& (facilities[this] == fac);
 
-predicate studentApplicationFields() = exists c:College,
-			camp:int, fac:IntCell, num:int ::
-			(this.college -> c) && (this.campusNumber -> camp) &&
-			(this.facilities -> fac) && (this.collegeNumber -> num)
-			
+procedure UnpackStudentApplicationFields(c:Ref, camp:int, fac:Ref, this:Ref);
+requires packedStudentApplicationFields[this];
+ensures (college[this] == c) && (campusNumber[this] == camp)
+	&& (facilities[this] == fac);
 
-predicate facilitiesOK() = exists f:IntCell, c:int :: 
-	this.facilities -> f && this.collegeNumber -> c &&
-	(f#1.0 MultipleOf(c))
+procedure PackStudentAppFacilitiesMany(col:Ref, c:int, f:Ref, this:Ref);
+requires packedStudentAppFacilitiesMany[this] == false;
+requires (college[this] == col) && (campusNumber[this] == c) &&
+	(facilities[this] == f) && 
+	packedCollegeFacilitiesMany[col] &&
+	(fracCollegeFacilitiesMany[col] == 1.0);
+//TODO add ensures about params in this object proposition
 
-void setStudentApplication(College college, int campusNumber) 
-requires this#1.0 studentApplicationFields()
-ensures this#1.0 facilitiesOK()
+procedure UnpackStudentAppFacilitiesMany(col:Ref, c:int, f:Ref, this:Ref);
+requires packedStudentAppFacilitiesMany[this];
+ensures (college[this] == col) && (campusNumber[this] == c) &&
+	(facilities[this] == f) && 
+	packedCollegeFacilitiesMany[col] &&
+	(fracCollegeFacilitiesMany[col] == 1.0);
+
+procedure PackStudentAppFacilitiesFew(col:Ref, c:int, f:Ref, this:Ref);
+requires packedStudentAppFacilitiesFew[this] == false;
+requires (college[this] == col) && (campusNumber[this] == c) &&
+	(facilities[this] == f) && 
+	packedCollegeFacilitiesFew[col] &&
+	(fracCollegeFacilitiesFew[col] == 1.0);
+//TODO add ensures about params in this object proposition
+
+procedure UnpackStudentAppFacilitiesFew(col:Ref, c:int, f:Ref, this:Ref);
+requires packedStudentAppFacilitiesFew[this];
+ensures (college[this] == col) && (campusNumber[this] == c) &&
+	(facilities[this] == f) && 
+	packedCollegeFacilitiesFew[col] &&
+	(fracCollegeFacilitiesFew[col] == 1.0);
+
+procedure ConstructStudentApplication(col:Ref, campusNum:int, this:Ref) 
+modifies college, facilities, campusNumber;
+ensures packedStudentApplicationFields[this] &&
+	(fracStudentApplicationFields[this] == 1.0)
 {
-		this.college = college;
-		this.campusNumber = campusNumber;
-		this.facilities = this.college.getNumberFacilities(campusNumber);
-		this.collegeNumber = this.college.getCollegeNumber();
+		college[this] := col;
+		call facilities[this] := getNumberFacilities(campusNum, college[this]);
+		campusNumber[this] := campusNum;	
+}
+	
+procedure changeApplicationFew(newCampusNumber:int, this:Ref)
+modifies campusNumber, facilities;
+requires packedStudentAppFacilitiesFew[this] &&
+	(fracStudentAppFacilitiesFew[this] == 1.0);
+ensures packedStudentAppFacilitiesFew[this] &&
+	(fracStudentAppFacilitiesFew[this] == 1.0);
+{
+	campusNumber[this] := modulo(newCampusNumber, 4);
+	call facilities[this] := getNumberFacilities(campusNumber[this], college[this]);
 }
 
-boolean checkNumberFacilities() 
-requires this#1.0 facilitiesOK()
-ensures this#1.0 facilitiesOK()
+procedure changeApplicationMany(newCampusNumber:int, this:Ref)
+modifies campusNumber, facilities;
+requires packedStudentAppFacilitiesMany[this] &&
+	(fracStudentAppFacilitiesMany[this] == 1.0);
+ensures packedStudentAppFacilitiesMany[this] &&
+	(fracStudentAppFacilitiesMany[this] == 1.0);
+{
+	campusNumber[this] := newCampusNumber * 10 + 1;
+	call facilities[this] := getNumberFacilities(campusNumber[this], college[this]);
+}
+
+
+procedure checkFacilitiesFew(this:Ref) returns (b:bool)
+requires packedStudentAppFacilitiesFew[this] &&
+	(fracStudentAppFacilitiesFew[this] == 1.0);
+ensures packedStudentAppFacilitiesFew[this] &&
+	(fracStudentAppFacilitiesFew[this] == 1.0);
 {        
-	return (this.facilities.getValueInt() % this.collegeNumber == 0);
-}
+	var temp:bool;
+	call temp := getValueInt(facilities[this]);
+	b := (temp <= 4 * campusNumber[this]);
 }
 
+procedure checkFacilitiesMany(this:Ref) returns (b:bool)
+requires packedStudentAppFacilitiesMany[this] &&
+	(fracStudentAppFacilitiesMany[this] == 1.0);
+ensures packedStudentAppFacilitiesMany[this] &&
+	(fracStudentAppFacilitiesMany[this] == 1.0);
+{       
+	var temp:bool;
+	call temp := getValueInt(facilities[this]);
+	b := (temp >= 10 * campusNumber[this]);
+}
 
